chore: adding more theory

Blase/Blase/MultiWidth/StreamDiffEq.lean
@@ -1,48 +1,170 @@
 import Blase.Fast.Circuit
 import Blase.Fast.FiniteStateMachine
 
+structure InputVar (ι : Type) (npast : Nat) where
+  input : ι
+  past : Fin npast
+deriving DecidableEq, Hashable
 
+private theorem Nat.mul_lt_mul_add {N M : Nat} {x y : Nat}
+    (hx : x < N) (hy : y < M) : x * M + y < N * M := by
+  have : 0 < N := by omega
+  have : N * M ≥ M := by
+    rcases N with rfl | N
+    · omega
+    · simp; rw [Nat.add_mul]; omega
+  have : y ≤ M - 1 := by omega
+  have : x * M ≤ N * M - M := by
+    apply le_sub_of_add_le
+    rw [← add_one_mul]
+    apply mul_le_mul_right
+    omega
+  have : x * M + y ≤ (N * M - M) + (M - 1) := by omega
+  have : x * M + y ≤ N * M - 1 := by
+    apply Nat.le_trans this
+    omega
+  omega
 
-inductive StreamVar (ι : Type) (npast : Nat) where
-| input (i : ι) (kpast : Fin npast) 
-| output (kpast : Fin npast) (h : 0 < kpast.val)
-deriving DecidableEq, Repr, Hashable
+@[simp]
+theorem FinEnum_card_eq_self :
+    FinEnum.card (Fin npast) = npast := by
+  simp only [FinEnum.card_fin]
 
-instance [DecidableEq ι] : FinEnum (StreamVar ι npast) where
-  card := sorry
-  equiv := sorry
+instance [instFinEnumI : FinEnum ι] : FinEnum (InputVar ι npast) where
+  card :=
+    let instFinEnumFinNpast : FinEnum (Fin npast) := by infer_instance
+    instFinEnumI.card * instFinEnumFinNpast.card
+  equiv := {
+    toFun := fun { input, past } =>
+      let instFinEnumFinNpast : FinEnum (Fin npast) := by infer_instance
+      let finInput := instFinEnumI.equiv.toFun input
+      let finPast := instFinEnumFinNpast.equiv.toFun past
 
--- out[0] = ...
--- a stream equation, that says that out[n] is a function of the inputs ι, and the previous outputs out[0], ..., out[n-1]
--- stream differential equation with 'ι' inputs, and 
+      ⟨finInput.val * instFinEnumFinNpast.card + finPast.val, by
+        apply Nat.mul_lt_mul_add
+        · sorry
+        · simp only [FinEnum.card_fin]
+          have := finPast.isLt
+          simpa using this
+      ⟩
+    invFun := fun x => sorry
+    left_inv := sorry
+    right_inv := sorry
+  }
+
 structure StreamDiffEq (ι : Type) (npast : Nat) where
-  -- | Assumed values of the output for the horizon.
-  outInit : (kpast : Fin npast) → (h : 0 < kpast.val) → Bool
-  -- | compute output as a function of past outputs and inputs
-  outCircuit : Circuit (StreamVar ι npast)
+  inInit : InputVar ι npast → Bool
+  outCircuit : Circuit (InputVar ι npast)
 
 
-def StreamDiffEq.toStream [DecidableEq ι] (s : StreamDiffEq ι npast) (input : ι → BitStream) : BitStream := 
-  let rec go (n : Nat) : Bool :=
-    if n < npast then
-      s.outInit (Fin.mk n (by omega)) (by omega)
-    else
-      let circInput : FinEnumVal (StreamVar ι npast) → Bool := 
-        fun v => match v with
-        | .input i kpast => input.get (n - kpast.val - 1)
-        | .output kpast h => go (n - kpast.val - 1)
-      s.outCircuit.eval circInput
-  ⟨go⟩
+/-- Cons a value onto a bitstream. -/
+def BitStream.cons (b : Bool) (bs : BitStream) : BitStream :=
+  fun n =>
+    match n with
+    | 0 => b
+    | n + 1 => bs n
 
-def StreamDiffEq.toFSM [DecidableEq ι] [Hashable ι] (s : StreamDiffEq ι npast) : FSM ι where
-  α := StreamVar ι npast
-  initCarry 
-    | .input i kpast => false
-    | .output kpast h => s.outInit kpast (by omega)
-  outputCirc := sorry
-  nextStateCirc := sorry
+@[simp]
+theorem BitStream.cons_zero (b : Bool) (bs : BitStream) :
+    (BitStream.cons b bs) 0 = b := rfl
+
+@[simp]
+theorem BitStream.cons_succ (b : Bool) (bs : BitStream) (n : Nat) :
+    (BitStream.cons b bs) (n + 1) = bs n := rfl
 
 
-    
+/-- Append n bits to the left of a bitstream. -/
+def BitStream.appendLeft (b : BitStream)
+    (n : Nat)
+    (env : Fin n → Bool) : BitStream :=
+    match n with
+    | 0 => b
+    | n + 1 => BitStream.cons (env 0) (b.appendLeft n (fun k => env k.succ))
+
+@[simp]
+theorem BitStream.appendLeft_zero (b : BitStream) (env : Fin 0 → Bool) :
+    b.appendLeft 0 env = b := rfl
 
 
+@[simp]
+theorem BitStream.appendLeft_succ (b : BitStream) (n : Nat)
+    (env : Fin (n + 1) → Bool) :
+    b.appendLeft (n + 1) env =
+      BitStream.cons (env 0) (b.appendLeft n (fun k => env k.succ)) := rfl
+
+@[simp]
+theorem BitStream.appendLeft_eq_ite (b : BitStream) (n : Nat)
+    (env : Fin n → Bool) (k : Nat) :
+    (b.appendLeft n env) k =
+      if h : k < n then env ⟨k, h⟩ else b (k - n) := by
+  induction n generalizing k with
+  | zero =>
+    simp [BitStream.appendLeft]
+  | succ n ihn =>
+    simp
+    induction k
+    case zero => simp
+    case succ k ihk =>
+      simp [ihn]
+
+/-- Lift a circuit to a bitstream by pointwise evaluation. -/
+def BitStream.ofCircuitPointwise(circ : Circuit α) (env : α → BitStream) : BitStream :=
+  fun n => circ.eval (fun a => env a n)
+
+@[simp]
+theorem eval_ofCircuitPointwise (circ : Circuit α) (env : α → BitStream) (n : Nat) :
+    (BitStream.ofCircuitPointwise circ env) n =
+      circ.eval (fun a => env a n) := rfl
+
+/-- Drop the first n bits of a bitstream. -/
+def BitStream.drop (bs : BitStream) (n : Nat) : BitStream :=
+  fun k => bs (k + n)
+
+@[simp]
+theorem BitStream.eval_drop (bs : BitStream) (n k : Nat) :
+    (BitStream.drop bs n) k = bs (k + n) := rfl
+
+/--
+Produce the output stream differential equation as a bitstream.
+-/
+def StreamDiffEq.toStream [DecidableEq ι]
+      (s : StreamDiffEq ι npast) (inputStream : ι → BitStream) : BitStream :=
+  let newStreams : ι → BitStream := fun i =>
+    BitStream.appendLeft (inputStream i) npast
+      (fun kpast => s.inInit ⟨i, kpast⟩)
+  BitStream.ofCircuitPointwise s.outCircuit fun iv =>
+    (newStreams iv.input).drop iv.past
+
+@[simp]
+theorem StreamDiffEq.toStream_eq_eval_of_lt [DecidableEq ι]
+    (s : StreamDiffEq ι npast)
+    (env : InputVar ι npast → Bool)
+    (inputStream : ι → BitStream) (n : Nat) (hn : ix < npast) :
+    (s.toStream inputStream) ix = s.outCircuit.eval env := by
+  simp [StreamDiffEq.toStream, BitStream.eval_drop]
+  congr
+  ext i
+  sorry
+
+/--
+Produce the output stream differential equation as a FSM
+-/
+def StreamDiffEq.toFSM [DecidableEq ι] [Hashable ι] [FinEnum ι]
+    (s : StreamDiffEq ι npast) : FSM ι where
+  α := InputVar ι npast
+  initCarry := s.inInit
+  outputCirc := s.outCircuit.map Sum.inl
+  -- | we need to rotate, and send bits to the more past state.
+  nextStateCirc := fun iv =>
+      if h : iv.past.val = 0 then
+        Circuit.var true <| .inr iv.input
+      else
+        Circuit.var true <| .inl ⟨iv.input, ⟨iv.past.val - 1, by omega⟩⟩
+
+theorem StreamDiffEq.toFsm_eval_eq_toStream [DecidableEq ι] [Hashable ι]
+    [FinEnum ι] (s : StreamDiffEq ι npast) (inputStream : ι → BitStream) :
+    (s.toFSM.eval inputStream) = (s.toStream inputStream) := by
+  ext i
+  by_cases hi : i < npast
+  · simp
+  · sorry
